\documentclass{article}
\usepackage[a4paper,margin=1cm]{geometry}
\usepackage{amsmath}
\title{Ä‡wiczenia 1}

\begin{document}
\maketitle

\begin{enumerate}
\item{}
    \begin{enumerate}
    \item{}
        \(7+4i+3(5-9i)=7+4i+15-27i=22-23i\)
    \item{}
        $Im(3+2i)(4-2i)-Re(5+3i)(1-4i)=2(4+2i)-5(1-4i)=8-4i-5-20=3+16i$
    \item{}
        $(3-2i)(3+4i)=9+12i-6i-8i^2=17+6i$
    \item{}
        $(4-5i)(4+5i)=4^2-(5i)^2=16+25=41$
    \item{}
        $\frac{-11+7i}{2+6i}=\frac{(-11+7i)(2-6i)}{(2+6i)(2-6i)}=\frac{-22+66i+14i-42i^2}{4+36}=\frac{20+80i}{40}=\frac{1}{2}+2i$
    \item{}
        $\frac{-1+2i}{5-3i}=\frac{(-1+2i)(5+3i)}{(5-3i)(5+3i)}=\frac{-5-3i+10i+6i^2}{25+9}=\frac{-11+7i}{31}=-\frac{11}{31}+\frac{7i}{31}$
    \item{}
        $\frac{3+i}{2-5i}=\frac{(3+i)(2+5i)}{(2-5i)(2+5i)}=\frac{6+15i+2i+5i^2}{4+25}=\frac{1+17i}{29}=\frac{1}{29}+\frac{17i}{29}$
    \item{}
        $\frac{5+3i}{8-2i}=\frac{(5+3i)(8+2i)}{(8-2i)(8+2i)}=\frac{40+10i+24i+6i^2}{64+4}=\frac{34+34i}{68}=\frac12+\frac12i$
    \item{}
        $\frac{3+2i}{-1+3i}=\frac{(3+2i)(-1-3i)}{(-1+3i)(-1-3i)}=\frac{-3-9i-2i-6i^2}{1+3}=\frac{3-11i}{4}=\frac34-\frac{11i}{4}$
    \end{enumerate}
\item{}
    \begin{enumerate}
    \item{}
        \begin{equation*}
        \left. \begin{aligned}
        2z+(3-i)\text{\={z}} &= 5+4i\\
        2(a+bi)+(3-i)(a-bi) &= 5+4i\\
        2a+2bi+3a-3bi-ai+bi^2 &= 5+4i \\
        5a-bi-ai-b &= 5+4i \\
        5a-b+i(-b-a)&=5+4i
        \end{aligned}
        \right \qquad \begin{aligned}
        5a-b&=5 \\
        -b-a&=4 \\
        a+b&=-4 \\
        b&=-4-a \\
        \\
        5a-(-4-a)&=5\\
        5a+4+a&=5\\
        6a&=1\\
        a&=\frac16\\
        \\
        b&=-4-\frac16\\
        b&=-\frac{25}{6}
        \end{aligned}
        \end{equation}
        \[z=\frac16-\frac{25}{6}i\]
    \item{}
    \end{enumerate}
\end{enumerate}
\end{document}
